PDDL_Relaxation.thy
@@ -3,6 +3,17 @@ imports "AI_Planning_Languages_Semantics.PDDL_STRIPS_Semantics"
     Formula_Normalization Utils AbLa_alts
 begin
 
+
+
+
+
+
+
+
+
+
+(* TODO: reevaluate the rest: *)
+
 context wf_ast_domain begin
                           
 fun relaxed_ac :: "ast_action_schema \<Rightarrow> bool" where
