Precondition_Normalization.thy
@@ -1,20 +1,9 @@
-theory Formula_Normalization
+theory Precondition_Normalization
 imports "AI_Planning_Languages_Semantics.PDDL_STRIPS_Semantics"
     Type_Normalization Utils AbLa_alts DNF
 begin
 
-
-locale type_normed_domain = wf_ast_domain +
-  assumes typeless_dom
-
-locale type_normed_problem = wf_ast_problem +
-  assumes "typeless_prob \<and> only_conj (goal P)"
-
 context ast_domain begin
-
-(* G for goal *)
-definition "dummy_pred \<equiv> Pred (safe_prefix pred_names @ ''G'')"
-definition "dummy_pred_decl \<equiv> PredDecl dummy_pred []"
 
 fun set_pre :: "ast_action_schema \<Rightarrow> term atom formula \<Rightarrow> ast_action_schema" where
   "set_pre (Action_Schema n params _ eff) pre = Action_Schema n params pre eff"
@@ -24,9 +13,6 @@ fun split_ac :: "ast_action_schema \<Rightarrow> ast_action_schema list" where
     map (set_pre ac) (dnf_list (ac_pre ac))"
 
 definition "split_acs \<equiv> concat (map split_ac (actions D))"
-
-fun dummy_ac where "dummy_ac (c, s) =
-  Action_Schema s [] c (Effect [Atom (predAtm dummy_pred [])] [])"
 
 abbreviation "ac_names \<equiv> map ac_name (actions D)"
 
