Tests.thy
@@ -3,87 +3,12 @@ theory Tests
     (* "../LTS-formalization/Datalog/Datalog"
     "AI_Planning_Languages_Semantics.PDDL_STRIPS_Semantics"
     "Verified_SAT_Based_AI_Planning.STRIPS_Representation"
-    "AI_Planning_Languages_Semantics.PDDL_STRIPS_Checker" *)
     "AI_Planning_Languages_Semantics.PDDL_STRIPS_Semantics"
     "HOL-Library.Monad_Syntax"
-    "HOL-Library.Multiset"
+    "HOL-Library.Multiset"*)
+    
+    "AI_Planning_Languages_Semantics.PDDL_STRIPS_Checker"
 begin
-
-thm valuation_iff_close_world
-thm valuation_def
-
-definition shave :: "world_model \<Rightarrow> world_model"
-  where "shave M \<equiv> {\<phi> \<in> M. is_predAtom \<phi>}"
-
-lemma "valuation (shave M) = valuation M"
-proof -
-  have "Atom (predAtm p xs) \<in> M \<longleftrightarrow> Atom (predAtm p xs) \<in> shave M" for p xs
-    using shave_def by simp
-  thus ?thesis using valuation_def by presburger
-qed
-
-term "(\<^sup>c\<TTurnstile>\<^sub>=)"
-
-
-
-
-term "count"
-
-
-datatype ('a, 'e) Err = Lef 'a | Rig 'e
-
-type_synonym ('a, 'e) err_ = "('a, 'e) Err" (infixl "#" 0)
-
-fun bind :: "('a # 'e) \<Rightarrow> ('a \<Rightarrow> ('b # 'e)) \<Rightarrow> ('b # 'e)" where
-  "bind (Lef x) f = f x"|
-  "bind (Rig e) f = Rig e"
-
-adhoc_overloading
-  Monad_Syntax.bind bind
-
-definition "dub x = Lef (x + x)"
-definition "odub x = Some (x + x)"
-
-value "(Rig False :: nat # bool) \<bind> dub"
-value "(None :: nat option) \<bind> odub"
-
-lemma "{x. \<exists>B \<in> s. x \<in> B} = \<Union>s" by auto
-lemma fixes a :: "'a set" shows "a \<bind> f = \<Union>(f ` a)"
-  by (rule Complete_Lattices.bind_UNION)
-
-(* ------------------------------------------------------------------------------------ *)
-
-lemma conj3: assumes "A \<and> B \<and> C" shows "A" "B" "C" using assms by simp_all
-
-lemma conj2: assumes "A \<and> B" shows "A" "B" using assms by simp_all
-
-lemma a: "(0::nat) < 3 \<and> (0::nat) < 6 \<and> (0::nat) < 9" by simp
-
-thm conj3[OF a]
-
-
-
-
-axiomatization f :: "('a \<times> 'a) list \<Rightarrow> ('a \<times> 'a) list" where
-  f_prop: "set (f rel) = (set rel)\<^sup>+"
-
-
-datatype slorp = Slorp (ann : nat) (ben : nat)
-
-fun gomp where "gomp (Slorp x y) = x + y"
-
-thm slorp.collapse
-
-lemma slorp_coll2: "\<lbrakk>\<And>x y. P (Slorp x y) x y\<rbrakk> \<Longrightarrow> P s (ann s) (ben s)"
-  by (metis slorp.collapse)
-
-lemma gomp2: "\<And>x y. gomp (Slorp x y) = x + y" by simp
-
-thm slorp_coll2[where P = "\<lambda>s x y. gomp s = x + y", OF gomp2]
-
-datatype 'a foom = Aned 'a 'a | Batt "'a list"
-
-value "map_foom (\<lambda>x :: nat. True)"
 
 
 
